Yes, a measurement where the measurement operators and the POVM elements coincide is a projective measurement. This can be proven by showing that the given condition forces the measurement operators to satisfy all the mathematical properties of a set of orthogonal projectors.

***

### **Question 7: Show that any measurement where the measurement operators and the POVM elements coincide is a projective measurement.**

### **1. Definitions**

Let's start by defining the key components of a general measurement and a projective measurement.

* **General Measurement (POVM):** A measurement is described by a set of **measurement operators** $\{M_m\}$, where $m$ corresponds to the measurement outcome.
    * The probability of outcome $m$ is $P(m) = \langle \psi | M_m^\dagger M_m | \psi \rangle$.
    * The operators must satisfy the **completeness relation**: $\sum_m M_m^\dagger M_m = I$.
    * The **POVM elements** are the positive operators $E_m \equiv M_m^\dagger M_m$.

* **Projective Measurement:** This is a special type of measurement where the measurement operators are a set of **projectors** $\{P_m\}$. A set of operators is a set of projectors if it satisfies:
    1.  **Hermiticity:** Each operator is Hermitian ($P_m^\dagger = P_m$).
    2.  **Idempotency:** Each operator squares to itself ($P_m^2 = P_m$).
    3.  **Orthogonality:** Projectors for different outcomes are orthogonal ($P_m P_k = 0$ for $m \neq k$).
    4.  **Completeness:** The projectors sum to the identity ($ \sum_m P_m = I$).

### **2. The Proof**

We are given the condition that the measurement operators and the POVM elements coincide for all outcomes $m$:

$$M_m = E_m$$

Using the definition of the POVM element, $E_m = M_m^\dagger M_m$, the condition becomes:

$$M_m = M_m^\dagger M_m$$

We will now use this central equation to prove that the set $\{M_m\}$ satisfies all four properties of a projective measurement.

---

#### **Step 1: Prove the Operators are Hermitian ($M_m^\dagger = M_m$)**
Let's take the Hermitian conjugate of our central equation:
$$M_m^\dagger = (M_m^\dagger M_m)^\dagger$$Using the property $(AB)^\dagger = B^\dagger A^\dagger$:$$M_m^\dagger = M_m^\dagger (M_m^\dagger)^\dagger = M_m^\dagger M_m$$We were given that $M_m^\dagger M_m = M_m$. Therefore:$$M_m^\dagger = M_m$$
This shows that each measurement operator $M_m$ is Hermitian. ✅

---

#### **Step 2: Prove the Operators are Idempotent ($M_m^2 = M_m$)**
Let's return to our central equation, $M_m = M_m^\dagger M_m$.
From Step 1, we know that we can replace the Hermitian conjugate $M_m^\dagger$ with $M_m$ itself:
$$M_m = (M_m) M_m = M_m^2$$
This shows that each measurement operator $M_m$ is idempotent. ✅

*At this point, we have proven that each operator $M_m$ is a projector. We will now rename them $P_m \equiv M_m$ and proceed to prove the properties of the complete set.*

---

#### **Step 3: Prove the Completeness Relation ($\sum_m P_m = I$)**
For any general measurement, the POVM elements must sum to the identity:
$$\sum_m E_m = I$$Since we are given that $M_m = E_m$, and we've established that $M_m = P_m$:$$\sum_m P_m = I$$
The set of projectors is complete. ✅

---

#### **Step 4: Prove the Operators are Orthogonal ($P_m P_k = 0$ for $m \neq k$)**
This property elegantly follows from the others. Let $P_k$ be any projector from the set. We can multiply it by the identity operator without changing it:
$$P_k = P_k I$$Now, substitute the completeness relation from Step 3 for $I$:$$P_k = P_k \left( \sum_m P_m \right) = \sum_m P_k P_m$$Let's split the sum into the case where $m=k$ and the cases where $m \neq k$:$$P_k = P_k P_k + \sum_{m \neq k} P_k P_m$$From Step 2, we know the projectors are idempotent ($P_k P_k = P_k^2 = P_k$).$$P_k = P_k + \sum_{m \neq k} P_k P_m$$Subtracting $P_k$ from both sides, we get:$$\sum_{m \neq k} P_k P_m = \mathbf{0}$$Now, consider any single term in this sum, $P_k P_m$. Let's pre-multiply this term by $P_k$:$$P_k (P_k P_m) = P_k^2 P_m = P_k P_m$$This doesn't simplify further. However, let's look at the sum again. A sum of positive semidefinite operators can only be zero if each term is zero. Let's show this applies. Consider the term $P_k P_m P_k$:$$(P_k P_m P_k) = (P_k P_m^{1/2})(P_m^{1/2}P_k)$$A clearer argument is as follows: Let $|\psi\rangle$ be any vector in the subspace corresponding to projector $P_m$. This means $P_m |\psi\rangle = |\psi\rangle$. We know that for any vector $|\psi\rangle$, its norm squared is equal to the sum of the norms of its projections onto the complete set of subspaces:$$||\psi||^2 = \sum_j ||P_j |\psi\rangle||^2$$In our case, since $|\psi\rangle$ is in the subspace of $P_m$, $P_m|\psi\rangle = |\psi\rangle$. This means:$$||\psi||^2 = ||P_m |\psi\rangle||^2 = ||\psi||^2$$Substituting this into the sum:$$||\psi||^2 = ||P_m |\psi\rangle||^2 + \sum_{j \neq m} ||P_j |\psi\rangle||^2 = ||\psi||^2 + \sum_{j \neq m} ||P_j |\psi\rangle||^2$$This implies that $\sum_{j \neq m} ||P_j |\psi\rangle||^2 = 0$. Since each term in the sum is non-negative, every individual term must be zero:$$||P_j |\psi\rangle||^2 = 0 \quad \text{for all } j \neq m$$This means $P_j |\psi\rangle = 0$. Since $|\psi\rangle = P_m |\psi\rangle$, we can write:$$P_j P_m |\psi\rangle = 0$$This holds for any vector $|\psi\rangle$, so we can conclude that the operator itself must be zero:$$P_j P_m = 0 \quad \text{for } j \neq m$$
The projectors are mutually orthogonal. ✅

**Conclusion:** We have shown that the given condition ($M_m = E_m$) forces the set of measurement operators $\{M_m\}$ to be a complete set of orthogonal projectors. A measurement described by such a set is, by definition, a **projective measurement**.