The observable $\vec{v} \cdot \vec{\sigma}$ has eigenvalues $\pm 1$. The matrices $P_\pm = \frac{I \pm \vec{v} \cdot \vec{\sigma}}{2}$ are indeed the correct projectors onto the corresponding eigenspaces. This is because the operator $\vec{v} \cdot \vec{\sigma}$ squares to the identity, a crucial property that dictates its eigenvalues and simplifies the verification of the projectors.

***

### **Question 4: Suppose $\vec{v}$ is any real three dimensional unit vector... Show that $\vec{v} \cdot \vec{\sigma}$ has eigenvalues $\pm 1$, and that the projectors onto the corresponding eigenspaces are given by $P_\pm = \frac{I \pm \vec{v} \cdot \vec{\sigma}}{2}$.**

Let's define the observable as $M \equiv \vec{v} \cdot \vec{\sigma}$. A key property of this operator, for any unit vector $\vec{v}$, is that it squares to the identity matrix:

$$M^2 = (\vec{v} \cdot \vec{\sigma})^2 = I$$

This identity is central to both parts of the proof.

---

## **Part 1: Finding the Eigenvalues**

We can find the eigenvalues of $M$ in two ways.

### **Solution 1.1: Using Operator Properties**

Let $\lambda$ be an eigenvalue of $M$ with a corresponding non-zero eigenvector $|\psi\rangle$. By definition:

$$M|\psi\rangle = \lambda|\psi\rangle$$

If we apply the operator $M$ a second time to this equation:

$$M^2|\psi\rangle = M(\lambda|\psi\rangle) = \lambda(M|\psi\rangle) = \lambda(\lambda|\psi\rangle) = \lambda^2|\psi\rangle$$

But we know that $M^2 = I$, so we also have:

$$M^2|\psi\rangle = I|\psi\rangle = |\psi\rangle$$

Equating our two expressions for $M^2|\psi\rangle$:

$$\lambda^2|\psi\rangle = |\psi\rangle$$

Since $|\psi\rangle$ is an eigenvector and thus non-zero, we can conclude:

$$\lambda^2 = 1 \implies \lambda = \pm 1$$

Thus, the only possible eigenvalues of the measurement are $+1$ and $-1$.

### **Solution 1.2: Using the Characteristic Equation**

First, we write out the matrix for $M$:

$$
M = v_1 X + v_2 Y + v_3 Z = \begin{pmatrix}
v_3 & v_1 - iv_2 \\\\
v_1 + iv_2 & -v_3
\end{pmatrix}
$$

The eigenvalues $\lambda$ are the roots of the characteristic equation $\det(M - \lambda I) = 0$:

$$
\det \begin{pmatrix}
v_3 - \lambda & v_1 - iv_2 \\\\
v_1 + iv_2 & -v_3 - \lambda
\end{pmatrix} = 0
$$

$$(v_3 - \lambda)(-v_3 - \lambda) - (v_1 - iv_2)(v_1 + iv_2) = 0$$$$-(v_3^2 - \lambda^2) - (v_1^2 + v_2^2) = 0$$$$\lambda^2 - v_3^2 - v_1^2 - v_2^2 = 0$$

Since $\vec{v}$ is a unit vector, $v_1^2 + v_2^2 + v_3^2 = 1$. The equation simplifies to:

$$\lambda^2 - 1 = 0 \implies \lambda = \pm 1$$

---

## **Part 2: Verifying the Projectors**

An operator $P$ is a **projector** onto an eigenspace of $M$ with eigenvalue $\lambda$ if it satisfies three properties:
1.  **Idempotent:** $P^2 = P$ (applying it twice is the same as applying it once).
2.  **Hermitian:** $P^\dagger = P$ (ensures the projection is orthogonal).
3.  **Projection Property:** $MP = \lambda P$ (it projects onto the correct eigenspace).

Let's verify these for $P_+ = \frac{I + M}{2}$ with eigenvalue $\lambda=+1$.

1.  **Idempotency:**
    $$
    P_+^2 = \left(\frac{I + M}{2}\right)^2 = \frac{1}{4}(I^2 + IM + MI + M^2)
    $$
    Using $M^2=I$, this becomes:
    $$
    P_+^2 = \frac{1}{4}(I + M + M + I) = \frac{1}{4}(2I + 2M) = \frac{I + M}{2} = P_+
    $$
2.  **Hermiticity:** $M$ is an observable and is therefore Hermitian ($M^\dagger = M$). The identity $I$ is also Hermitian. A linear combination of Hermitian operators with real coefficients is Hermitian, so $P_+$ is Hermitian.

3.  **Projection Property:**
    $$
    MP_+ = M\left(\frac{I + M}{2}\right) = \frac{1}{2}(MI + M^2) = \frac{1}{2}(M + I) = P_+
    $$
    This is equivalent to $MP_+ = (+1)P_+$.

All three properties hold for $P_+$. The verification for $P_- = \frac{I - M}{2}$ with eigenvalue $\lambda=-1$ follows the same logic.

1.  **Idempotency:**
    $$
    P_-^2 = \left(\frac{I - M}{2}\right)^2 = \frac{1}{4}(I^2 - IM - MI + M^2) = \frac{1}{4}(I - 2M + I) = \frac{I - M}{2} = P_-
    $$
2.  **Hermiticity:** $P_-$ is also Hermitian for the same reason as $P_+$.

3.  **Projection Property:**
    $$
    MP_- = M\left(\frac{I - M}{2}\right) = \frac{1}{2}(MI - M^2) = \frac{1}{2}(M - I) = -\left(\frac{I - M}{2}\right) = -P_-
    $$
    This is equivalent to $MP_- = (-1)P_-$.

All properties hold, confirming that $P_\pm$ are the correct projectors. üèõÔ∏è